updated to move to ET

ContractExamples/FStar/CallOption.fst
@@ -4,6 +4,7 @@ open Zen.Base
 open Zen.Cost
 open Zen.Types
 open Zen.Merkle
+open Zen.ErrorT
 open FStar.UInt64
 
 module M = FStar.Mul
@@ -25,7 +26,7 @@ let (-?^) x y = ET.of_option "Overflow Error" (U64.checked_sub x y)
 val ( *?^ ): U64.t -> U64.t -> cost (result U64.t) 4
 let ( *?^ ) x y = ET.of_option "Overflow Error" (U64.checked_mul x y)
 
-let numeraire: cost hash 3 = ret @ Zen.Util.hashFromBase64 "AAAAAAAAAAAAAAAAAAAAAAAAAAAAAAAAAAAAAAAAAAA="
+let numeraire: cost (result hash) 3 = ret @ Zen.Util.hashFromBase64 "AAAAAAAAAAAAAAAAAAAAAAAAAAAAAAAAAAAAAAAAAAA="
 
 // "price" is the premium, in kalapas
 let price: U64.t = 100UL
@@ -33,7 +34,7 @@ let price: U64.t = 100UL
 // strike in u64 is real strike * 1000, rounded down
 let strike: U64.t = 1000000UL
 
-let oracleHash: cost hash 3 = ret @ Zen.Util.hashFromBase64 "AAAAAAAAAAAAAAAAAAAAAAAAAAAAAAAAAAAAAAAAAAA="
+let oracleHash: cost (result hash) 3 = ret @ Zen.Util.hashFromBase64 "AAAAAAAAAAAAAAAAAAAAAAAAAAAAAAAAAAAAAAAAAAA="
 
 // No string -> byte arrays, yet. So 32 byte arrays to represent
 // the underlying, i.e. stuff like "AAPL", "MSFT", etc. To use:
@@ -46,10 +47,9 @@ let underlyingSymbol = ret @ Zen.Util.hashFromBase64
 type pointedOutput = outpoint * output
 
 val tryAddPoint: outpoint -> utxos:utxo -> cost (result pointedOutput) 7
-let tryAddPoint pt utxos = let open ET in
-  match utxos pt with
-  | Some oput -> ret (pt, oput)
-  | None -> failw "Cannot find output in UTXO set"
+let tryAddPoint pt utxos = match utxos pt with
+                           | Some oput -> ret (pt, oput)
+                           | None -> failw "Cannot find output in UTXO set"
 
 type oracleData (n:nat) = { underlying: Zen.Array.t byte n;
                             price : U64.t;
@@ -98,7 +98,7 @@ type dcommand (iMsg:inputMsg) = dcmd:command // Command that depends on input me
     | _ -> Fail? dcmd }
 
 val makeCommand : iMsg:inputMsg -> cost (dcommand iMsg) 72
-let makeCommand iMsg = let open M in
+let makeCommand iMsg = let open Zen.Cost in
   match iMsg with
   | { cmd=0uy; data=(| _, Outpoint pt |) }->
       ret@Initialize pt
@@ -142,11 +142,11 @@ type state = { tokensIssued : U64.t;
 val encodeState : state -> cost (inputData 3) 10
 let encodeState { tokensIssued=tokensIssued;
                   collateral=collateral;
-                  counter=counter } =
+                  counter=counter } = let open Zen.Cost in
     ret @ UInt64Vector 3 V[tokensIssued; collateral; counter]
 
 val decodeState : #n:nat -> inputData n -> cost (result state) 16
-let decodeState #n iData = let open ET in
+let decodeState #n iData =
   if n <> 3 then autoFailw "Bad data" else
   match iData with
   | UInt64Vector 3 V[tk; coll; cter] ->
@@ -154,16 +154,15 @@ let decodeState #n iData = let open ET in
   | _ -> autoFailw "Bad data"
 
 val findRoot : #n:nat -> inputData n -> #nAuditPathHashes:nat -> (path:auditPath nAuditPathHashes)
-    -> cost (result hash) M.(n * 384 + 1064 + nAuditPathHashes)
+    -> cost (result hash) M.(n * 384 + 1059 + nAuditPathHashes)
 let findRoot #n iData #nAuditPathHashes {location=location;hashes=hashes} =
   let inputHash = hashData iData in
   let optRoot = OT.bindLift inputHash (function h -> rootFromAuditPath h location hashes) in
-  do optRoot' <-- optRoot;
-  ret @ O.maybe (E.failw "Can't hash input data") (E.ret) optRoot'
+  ET.of_optionT "Can't hash input data" optRoot
 
-val initializeTx : utxo -> hash -> outpoint -> cost (result transactionSkeleton) 56
-let initializeTx utxo cHash outpoint = let open ET in
-    do numeraire <-- retT numeraire;
+val initializeTx : utxo -> hash -> outpoint -> cost (result transactionSkeleton) 55
+let initializeTx utxo cHash outpoint =
+    do numeraire <-- numeraire;
     do (pt, oput) <-- tryAddPoint outpoint utxo;
     if oput.spend.asset <> numeraire
     then autoFailw "Can't initialize with this asset." else     // Initialize with data output
@@ -180,9 +179,9 @@ val collateralizeTx: utxo
                      -> hash
                      -> outpoint
                      -> outpoint
-                     -> cost (result transactionSkeleton) 128
-let collateralizeTx utxo cHash outpoint0 outpoint1 = let open ET in
-    do numeraire <-- retT numeraire;
+                     -> cost (result transactionSkeleton) 127
+let collateralizeTx utxo cHash outpoint0 outpoint1 =
+    do numeraire <-- numeraire;
     do (pt0, dataOutput)     <-- tryAddPoint outpoint0 utxo;
     do (pt1, newFundsOutput) <-- tryAddPoint outpoint1 utxo;
     if dataOutput.spend.asset <> numeraire || newFundsOutput.spend.asset <> numeraire
@@ -211,9 +210,9 @@ val buyTx: utxo
            -> outpoint
            -> outpoint
            -> outputLock
-           -> cost (result transactionSkeleton) 143
-let buyTx utxo cHash outpoint0 outpoint1 lk = let open ET in
-    do numeraire <-- retT numeraire;
+           -> cost (result transactionSkeleton) 142
+let buyTx utxo cHash outpoint0 outpoint1 lk =
+    do numeraire <-- numeraire;
     do (pt0, dataOutput)     <-- tryAddPoint outpoint0 utxo;
     do (pt1, purchaseOutput) <-- tryAddPoint outpoint1 utxo;
     if dataOutput.spend.asset <> numeraire || purchaseOutput.spend.asset <> numeraire
@@ -243,12 +242,12 @@ let buyTx utxo cHash outpoint0 outpoint1 lk = let open ET in
 val restOfEx: hash -> pointedOutput -> pointedOutput -> pointedOutput
               -> U64.t
               -> outputLock
-              -> cost (result transactionSkeleton) 135
+              -> cost (result transactionSkeleton) 134
 let restOfEx cHash
              (pt1,dataOutput) (pt2,tokenOutput) (pt3,oracleOutput)
              spot
-             payoffOutputLock = let open ET in
-    do numeraire <-- retT numeraire;
+             payoffOutputLock =
+    do numeraire <-- numeraire;
     if dataOutput.spend.asset <> numeraire || tokenOutput.spend.asset <> cHash
     then autoFailw "Can't exercise with these assets." else
     match dataOutput.lock, tokenOutput.lock with
@@ -286,7 +285,7 @@ val exerciseTx: utxo -> hash
                 -> (path:auditPath nAuditPathHashes)
                 -> outputLock
                 -> cost (result transactionSkeleton)
-                         M.((nUnderlyingAssetBytes+3) * 384 + 1302 + nAuditPathHashes)
+                         M.((nUnderlyingAssetBytes+3) * 384 + 1292 + nAuditPathHashes)
 let exerciseTx utxo
                cHash
                outpoint0 outpoint1 outpoint2
@@ -297,7 +296,7 @@ let exerciseTx utxo
                  nonce=nonce }
                #nAuditPathHashes
                auditPath
-               payoffOutputLock = let open ET in
+               payoffOutputLock =
     do (pt0, dataOutput)   <-- tryAddPoint outpoint0 utxo;
     do (pt1, tokenOutput)  <-- tryAddPoint outpoint1 utxo;
     do (pt2, oracleOutput) <-- tryAddPoint outpoint2 utxo;
@@ -312,13 +311,13 @@ let exerciseTx utxo
     match oracleOutput with
     | { lock=(ContractLock oHash 1 (Hash mroot));
         spend={asset=oHash2} } ->
-          do oracleHash <-- retT @ oracleHash;
+          do oracleHash <-- oracleHash;
           if oHash <> oracleHash then autoFailw "Incorrect oracle ID" else
           if oHash2 <> oracleHash then autoFailw "Wrong oracle asset type" else
           if not (expectedRoot = mroot) then autoFailw "wrong root" else
           if nUnderlyingAssetBytes <> 32
           then autoFailw "Limitation: symbol must be 32 bytes." else begin
-          do underlyingSymbol <-- retT @ underlyingSymbol;
+          do underlyingSymbol <-- underlyingSymbol;
           if underlyingBytes <> underlyingSymbol
           then autoFailw "Trying to use the wrong underlying!" else
           restOfEx cHash
@@ -330,18 +329,18 @@ let exerciseTx utxo
 
 val cf': inputMsg -> nat -> cost nat 58
 let cf' iMsg k = let open M in
-  ret (k +
+  Zen.Cost.ret (k +
   begin match iMsg with
-  | { cmd = 0uy ; data = (| _ , Outpoint pt |) } -> 56
-  | { cmd = 1uy ; data = (| _ , OutpointVector 2 _ |) } -> 128
-  | { cmd = 2uy ; data = (| _ , Data2 _ _ (OutpointVector 2 _) (OutputLock lk) |) } -> 143
+  | { cmd = 0uy ; data = (| _ , Outpoint pt |) } -> 55
+  | { cmd = 1uy ; data = (| _ , OutpointVector 2 _ |) } -> 127
+  | { cmd = 2uy ; data = (| _ , Data2 _ _ (OutpointVector 2 _) (OutputLock lk) |) } -> 142
   | { cmd = 3uy ;
       data=(| _, Data4 _ _ _ _
                    _
                    (Data4 _ _ _ _ (ByteArray nUnderlyingAssetBytes _) _ _ _)
                    (Data2 _ _ _ (HashArray nAuditPathHashes _))
                    _ |) } ->
-                     (nUnderlyingAssetBytes + 3) * 384 + 1302 + nAuditPathHashes
+                     (nUnderlyingAssetBytes + 3) * 384 + 1292 + nAuditPathHashes
   | _ -> 0
   end)
 
@@ -351,16 +350,16 @@ let cf i = cf' i 105
 val cf_lemma: i:inputMsg -> Lemma (let open M in
    force (cf i) == 105 +
    begin match i with
-   | { cmd = 0uy ; data = (| _ , Outpoint pt |) } -> 56
-   | { cmd = 1uy ; data = (| _ , OutpointVector 2 _ |) } -> 128
-   | { cmd = 2uy ; data = (| _ , Data2 _ _ (OutpointVector 2 _) (OutputLock lk) |) } -> 143
+   | { cmd = 0uy ; data = (| _ , Outpoint pt |) } -> 55
+   | { cmd = 1uy ; data = (| _ , OutpointVector 2 _ |) } -> 127
+   | { cmd = 2uy ; data = (| _ , Data2 _ _ (OutpointVector 2 _) (OutputLock lk) |) } -> 142
    | { cmd = 3uy ;
        data=(| _, Data4 _ _ _ _
                     _
                     (Data4 _ _ _ _ (ByteArray nUnderlyingAssetBytes _) _ _ _)
                     (Data2 _ _ _ (HashArray nAuditPathHashes _))
                     _ |) } ->
-                      (nUnderlyingAssetBytes + 3) * 384 + 1302 + nAuditPathHashes
+                      (nUnderlyingAssetBytes + 3) * 384 + 1292 + nAuditPathHashes
    | _ -> 0
    end)
 let cf_lemma = function
@@ -377,6 +376,7 @@ let cf_lemma = function
 
 val main : i:inputMsg -> cost (result transactionSkeleton) (force (cf i))
 let main i = let open M in
+             let open Zen.Cost in
   cf_lemma i;
   do command <-- makeCommand i;
   match command with
@@ -384,16 +384,16 @@ let main i = let open M in
       initializeTx i.utxo i.contractHash pointed
       <: cost (result transactionSkeleton)
          (match i with
-          | { cmd = 0uy ; data = (| _ , Outpoint pt |) } -> 56
-          | { cmd = 1uy ; data = (| _ , OutpointVector 2 _ |) } -> 128
-          | { cmd = 2uy ; data = (| _ , Data2 _ _ (OutpointVector 2 _) (OutputLock lk) |) } -> 143
+          | { cmd = 0uy ; data = (| _ , Outpoint pt |) } -> 55
+          | { cmd = 1uy ; data = (| _ , OutpointVector 2 _ |) } -> 127
+          | { cmd = 2uy ; data = (| _ , Data2 _ _ (OutpointVector 2 _) (OutputLock lk) |) } -> 142
           | { cmd = 3uy ;
               data=(| _, Data4 _ _ _ _
                            _
                            (Data4 _ _ _ _ (ByteArray nUnderlyingAssetBytes _) _ _ _)
                            (Data2 _ _ _ (HashArray nAuditPathHashes _))
                            _ |) } ->
-                             (nUnderlyingAssetBytes + 3) * 384 + 1302 + nAuditPathHashes
+                             (nUnderlyingAssetBytes + 3) * 384 + 1292 + nAuditPathHashes
           | _ -> 0)
   | Collateralize V[pointed ; pointed'] ->
       collateralizeTx i.utxo i.contractHash pointed pointed'
@@ -402,4 +402,4 @@ let main i = let open M in
   | Exercise V[ptd ; ptd' ; ptd''] nUnderlyingAssetBytes d nAuditPathHashes path lk ->
       exerciseTx i.utxo i.contractHash ptd ptd' ptd'' d path lk
   | Fail msg ->
-      ET.failw msg
+      failw msg
